\documentclass[11pt,letterpaper,titlepage]{article}

\usepackage{geometry}
\geometry{left=1.5cm,right=1.5cm,top=1.5cm,bottom=2.5cm}

\usepackage{setspace}
\onehalfspacing

\usepackage{fancyhdr}

\usepackage{amsmath}

\usepackage{amssymb}

\usepackage{booktabs}

\usepackage{pifont}

\pagestyle{fancy}
\lhead{}
\rhead{}
\lfoot{ECEN 662 Estimation and Detection Theory}
\cfoot{\thepage}
\rfoot{Assignment 2 @Lei Wang}
\renewcommand{\headrulewidth}{0pt}
\renewcommand{\headwidth}{\textwidth}
\renewcommand{\footrulewidth}{0.4pt}
\newcommand{\RomanNumeralCaps}[1]
    {\MakeUppercase{\romannumeral #1}}

\begin{document}

\begin{enumerate}
    \item %Q1
    
    \begin{equation*}
        \begin{aligned}
            E[X] &= \int_{\infty}^{\infty} x f_X(x) dx \\
            &= \int_{-\infty}^{x} u \cdot 0 du + \int_{x}^{\infty} u \frac{1}{\sqrt{2\pi}} e^{-\frac{u^2}{2}} du \\
            &= -\frac{1}{\sqrt{2\pi}} e^{-\frac{u^2}{2}} |_{x}^{\infty} \\
            &= \frac{1}{\sqrt{2\pi}} e^{-\frac{x^2}{2}}
        \end{aligned}
    \end{equation*}
    
    \item %Q2
    
    \begin{enumerate}
        \item 
        
        \item
        
    \end{enumerate}
    
    \item %Q3
    
    \begin{enumerate}
        \item 
        
        \item
        
    \end{enumerate}
    
    \item %Q4
    
    The probability that a continuous random variable is greater than its expectation is $\frac{1}{2}$.
    
    Therefore, $Y_i$s are binomial random variables with the following parameters:
    
    \begin{gather*}
        \begin{cases}
        Pr(Y_i = 1) = \frac{1}{2} \\
        Pr(Y_i = 0) = \frac{1}{2}
        \end{cases}
    \end{gather*}

    Hence the distribution of the sum of $Y_i$s is the following:
    
    \begin{equation*}
        Pr(\sum_{i = 1}^{n} Y_i = k) = {n \choose k} \frac{1}{2^n}, k \in [0, n] \text{ and } k \in \mathbb{Z}
    \end{equation*}
    
    
    \item %Q5
    
    \item %Q6
    
    \begin{enumerate}
        \item 
        
        \begin{equation*}
            \begin{aligned}
                \overline{X_n} &= \frac{1}{n} \sum_{i = 1}^{n} X_i \\
                \sum_{i = 1}^{n} X_i &= n \overline{X_n} \\
                \sum_{i = 1}^{n} X_i + X_{n+1} &= n \overline{X_n} + X_{n+1} \\
                \sum_{i = 1}^{n+1} X_i &= n \overline{X_n} + X_{n+1} \\
                \frac{1}{n + 1} \sum_{i = 1}^{n+1} X_i &= \frac{n \overline{X_n} + X_{n+1}}{n + 1} \\
                \overline{X_{n + 1}} &= \frac{n \overline{X_n} + X_{n+1}}{n + 1}
            \end{aligned}
        \end{equation*}
        
        \item
        
        \begin{equation*}
            \begin{aligned}
                S_n^2 & = \frac{1}{n-1} \sum_{i=1}^{n} (X_i - \overline{X_n})^2 \\
                S_{n+1}^2 & = \frac{1}{n} \sum_{i=1}^{n+1} (X_i - \overline{X_{n+1}})^2 \\
                n S_{n+1}^2 &= (n - 1) S_n^2 + \sum_{i=1}^{n+1} (X_i - \overline{X_{n+1}})^2 - \sum_{i=1}^{n} (X_i - \overline{X_n})^2 \\
                n S_{n+1}^2 &= (n - 1) S_n^2 + (X_{n + 1} - \overline{X_{n+1}})^2 + \sum_{i=1}^{n} (X_i - \overline{X_{n+1}})^2 - \sum_{i=1}^{n} (X_i - \overline{X_n})^2 \\
                n S_{n+1}^2 &= (n - 1) S_n^2 + (X_{n + 1} - \overline{X_{n+1}})^2 + \sum_{i=1}^{n} [(X_i - \overline{X_{n+1}})^2 - (X_i - \overline{X_n})^2] \\
                n S_{n+1}^2 &= (n - 1) S_n^2 + (X_{n + 1} - \overline{X_{n+1}})^2 + \sum_{i=1}^{n} [X_i^2 - 2 X_i \overline{X_{n+1}} + \overline{X_{n+1}}^2 - X_i^2 + 2 X_i \overline{X_{n}} - \overline{X_{n}}^2] \\
                n S_{n+1}^2 &= (n - 1) S_n^2 + (X_{n + 1} - \overline{X_{n+1}})^2 + \sum_{i=1}^{n} [- 2 X_i \overline{X_{n+1}} + \overline{X_{n+1}}^2 + 2 X_i \overline{X_{n}} - \overline{X_{n}}^2] \\
                n S_{n+1}^2 &= (n - 1) S_n^2 + (X_{n + 1} - \overline{X_{n+1}})^2 + n \overline{X_{n+1}}^2 - n \overline{X_{n}}^2 + (- 2 \overline{X_{n+1}} + 2 \overline{X_{n}}) \sum_{i=1}^{n} [X_i ] \\
                n S_{n+1}^2 &= (n - 1) S_n^2 + (X_{n + 1} - \overline{X_{n+1}})^2 + n \overline{X_{n+1}}^2 - n \overline{X_{n}}^2 + (- 2 \overline{X_{n+1}} + 2 \overline{X_{n}}) n \overline{X_n} \\
                n S_{n+1}^2 &= (n - 1) S_n^2 + (X_{n + 1} - \overline{X_{n+1}})^2 + n \overline{X_{n+1}}^2 + n \overline{X_{n}}^2 - 2 n \overline{X_n} \overline{X_{n+1}} \\
                n S_{n+1}^2 &= (n - 1) S_n^2 + (X_{n + 1} - \overline{X_{n+1}})^2 + n (\overline{X_n} - \overline{X_{n+1}})^2 \text{, use the answer in a)}\\
                n S_{n+1}^2 &= (n - 1) S_n^2 + (X_{n + 1} - \frac{n \overline{X_n} + X_{n+1}}{n + 1})^2 + n (\overline{X_n} - \frac{n \overline{X_n} + X_{n+1}}{n + 1})^2 \\
                n S_{n+1}^2 &= (n - 1) S_n^2 + (\frac{(n + 1)X_{n+1} - n \overline{X_n} - X_{n+1}}{n+1})^2 + n (\frac{(n + 1) \overline{X_n} - n \overline{X_n} - X_{n+1}}{n+1})^2 \\
                n S_{n+1}^2 &= (n - 1) S_n^2 + (\frac{n X_{n+1} - n \overline{X_n}}{n+1})^2 + n (\frac{\overline{X_n} - X_{n+1}}{n+1})^2 \\
                n S_{n+1}^2 &= (n - 1) S_n^2 + \frac{n}{(n + 1)^2} (n \overline{X_{n+1}}^2 - 2 n X_{n+1} \overline{X_n} + n \overline{X_n}^2 + \overline{X_n}^2 - 2 X_{n+1} \overline{X_n} + \overline{X_n}^2) \\
                 n S_{n+1}^2 &= (n - 1) S_n^2 + \frac{n}{(n + 1)^2} (n + 1) (\overline{X_{n+1}}^2 - 2 X_{n+1} \overline{X_n} + \overline{X_n}^2) \\
                 n S_{n+1}^2 &= (n - 1) S_n^2  + \frac{n}{n + 1} (X_{n+1} - \overline{X_n}^2)^2
            \end{aligned}
        \end{equation*}
        
    \end{enumerate}
    
\end{enumerate}

\end{document}
